coq/SigmaHCOL/MemVecEq.v
@@ -477,6 +477,32 @@ Section MemVecEq.
       | List.cons hd tl => Add A (set_of_list tl) hd
       end.
 
+  Lemma mem_try_add_None (m:mem_block) {kv}:
+    NM.In (fst kv) m -> mem_try_add m kv ≡ None.
+  Proof.
+    intros H.
+    unfold mem_try_add.
+    break_let.
+    break_if.
+    -
+      reflexivity.
+    -
+      simpl in H.
+      congruence.
+  Qed.
+
+  Lemma mem_try_add_Some (m:mem_block) {k:NM.key} {v:CarrierA}:
+    not (NM.In k m) -> mem_try_add m (k,v) ≡ Some (NM.add k v m).
+  Proof.
+    intros H.
+    unfold mem_try_add.
+    break_if.
+    -
+      congruence.
+    -
+      reflexivity.
+  Qed.
+
   (* TODO: could be proven <-> *)
   Lemma mem_merge_is_Some
         (m0 m1 : mem_block)
@@ -509,6 +535,7 @@ Section MemVecEq.
   Proof.
   Admitted.
 
+  (* TODO: move somewhere in Memory *)
   Lemma mem_merge_contains_1st
         (m m0 m1 : mem_block)
         (MM : mem_merge m0 m1 ≡ Some m)
@@ -518,7 +545,7 @@ Section MemVecEq.
   Admitted.
 
 
-    (* TODO: move somewhere in Memory *)
+  (* TODO: move somewhere in Memory *)
   Lemma mem_merge_contains_2nd
         (m m0 m1 : mem_block)
         (MM : mem_merge m0 m1 ≡ Some m)
@@ -552,8 +579,15 @@ Section MemVecEq.
 
   Admitted.
 
+  (* Too general try same for `fold` *)
+  Lemma elements_add_new {A:Type} (v:A) {m k}:
+    not (NM.In k m) ->
+    NM.elements (NM.add k v m) ≡ List.cons (k,v) (NM.elements m).
+  Proof.
+  Admitted.
+
   (* TODO: move somewhere in Memory *)
-  Lemma mem_merge_key_either
+  Lemma mem_merge_key_dec
         (m m0 m1 : mem_block)
         (MM : mem_merge m0 m1 ≡ Some m)
     :
@@ -561,42 +595,51 @@ Section MemVecEq.
   Proof.
     intros k H.
     rename m into mm, k into kk.
-    rewrite mem_block_elements with (m:=m0).
-    generalize dependent (NM.elements m0).
-    revert MM.
-    intros l MM.
-
-
-
-    
-    destruct (NF.In_dec m1 kk) as [M1 | M1].
+    destruct (NF.In_dec m1 kk) as [M1 | M1], (NF.In_dec m0 kk) as [M0|M0].
+    -
+      right.
+      apply M1.
     -
       right.
       apply M1.
     -
       left.
-      dependent induction l.
+      apply M0.
+    -
+      exfalso. (* Could not be in neither. *)
+      rewrite mem_block_elements with (m:=m0) in *.
+      unfold mem_merge in MM.
+      pose proof (NM.elements_3w m0) as U0.
+      generalize dependent (NM.elements m0). intros ll0 MM MM0 U0.
+      clear m0.
+
+      induction ll0.
       +
-        simpl in *.
-        some_inv.
         crush.
       +
-        destruct a as [k' v].
+        destruct a as [k v].
         simpl in *.
-        destruct (eq_nat_dec k' kk) as [K|NK].
+        destruct (eq_nat_dec k kk) as [K|NK].
         *
-          (* k in m1 *)
-          apply NF.add_in_iff.
-          auto.
+          (* k=kk *)
+          contradict MM0.
+          apply NF.add_in_iff; auto.
         *
-          apply NF.add_neq_in_iff. apply NK.
-          apply IHl; clear IHl; try auto.
-          break_match_hyp; try break_if; try some_none.
-          some_inv.
-          subst mm.
-          apply NF.add_neq_in_iff in H; auto.
-          apply NF.not_mem_in_iff in Heqb.
-
+          apply IHll0; clear IHll0.
+          --
+            (* rewrite elements_add_new in MM. *)
+            clear kk M1 MM0 NK H.
+            rewrite <- MM; clear MM.
+            inversion_clear U0.
+            f_equiv.
+            f_equiv.
+            admit.
+          --
+            rewrite NF.add_neq_in_iff in MM0 by auto.
+            apply MM0.
+          --
+            inversion_clear U0.
+            auto.
   Admitted.
 
   (* TODO: move somewhere in Utils *)
